hol/functional/compiler_evalScript.sml
@@ -1,10 +1,11 @@
+Theory compiler_eval
+Ancestors
+  arithmetic list pair finite_map string
+  words compiler_prog compiler_funs_cv
+Libs
+  cv_transLib wordsLib automationLib
 
-open HolKernel Parse boolLib bossLib term_tactic;
-open arithmeticTheory listTheory pairTheory finite_mapTheory stringTheory;
-open wordsTheory wordsLib automationLib compilerTheory compiler_progTheory;
-
-val _ = new_theory "compiler_eval";
-
+val _ = max_print_depth := 10;
 
 Definition compiler_str_def:
   compiler_str = prog2str compiler_prog coms
@@ -18,12 +19,15 @@ Definition compiler_asm_str_def:
   compiler_asm_str = asm2str compiler_asm
 End
 
-Theorem compiler_str      = time EVAL “compiler_str”;
-Theorem compiler_asm      = time EVAL “compiler_asm”;
-Theorem compiler_asm_str  = time EVAL “compiler_asm_str”;
+val _ = cv_trans_deep_embedding EVAL compiler_prog_def;
+val _ = cv_trans coms_def;
+val _ = cv_trans compiler_str_def;
+val _ = cv_trans compiler_asm_def;
+val _ = cv_trans compiler_asm_str_def;
+
+Theorem compiler_str      = time cv_eval “compiler_str”;
+Theorem compiler_asm      = time cv_eval “compiler_asm”;
+Theorem compiler_asm_str  = time cv_eval “compiler_asm_str”;
 
 val _ = write_hol_string_to_file "compiler_prog.txt" (compiler_str |> concl |> rand);
 val _ = write_hol_string_to_file "compiler_asm.s"    (compiler_asm_str |> concl |> rand);
-
-
-val _ = export_theory();
